WIP

Clap/Lang/FB/assert.lean
@@ -1,12 +1,41 @@
 import Clap.Lang.FB.FB
 import Clap.Lang.FB.not
-import Clap.eDSLState.Basic
+
+import Clap.eDSLState.Writer
+import Clap.eDSLState.Wheels
 
 namespace Clap.Lang.FB
 
 def assert {p : ℕ} [Fact (p ≥ 2)] (a : FB p) : Edsl.CircuitStateM p Unit := do
   Edsl.eq0 (not a)
 
+namespace assert
 
+-- TODO do we need a relation between varStore and numAlloc
+-- perhaps that varStore is full up to numAlloc?
+def matchesUnaryPredicatePure
+  (p : ℕ)
+  (spec_function : Bool → Prop)
+  (function : FB p → Edsl.CircuitStateM p Unit)
+: Prop :=
+  ∀ (a : FB p) varStore numAlloc, a.isValid (varStore.get?) →
+    let ⟨numAllocPost, varStorePost, constraints⟩ := Edsl.CircuitState.eval
+      ((function a).run numAlloc).1.2
+      varStore
+      numAlloc
+    constraints = spec_function (a.toBool varStore.get?) ∧
+    numAllocPost = numAlloc ∧
+    varStorePost = varStore
+
+def spec (p : ℕ) [Fact (p ≥ 2)] : Prop := matchesUnaryPredicatePure p (·) FB.assert
+
+lemma equiv {p : ℕ} [Fact (p ≥ 2)] :
+  spec p
+:= by
+  intro a varStore numAlloc h_isValid
+  simp [Clap.monads, FB.assert]
+  done
+
+end assert
 
 end Clap.Lang.FB
