Clap/Lang/FB/not.lean
@@ -8,42 +8,14 @@ namespace not
 
 def spec (p : ℕ) [Fact (p ≥ 2)] : Prop := matchesUnaryFunction p (!·) FB.not
 
-lemma equiv {p : ℕ} [Fact (p ≥ 2)] : spec p
+lemma equiv {p : ℕ} [Fact (p ≥ 2)] :
+  spec p
 := by
   intro a varStore h_isValid
-  have : p ≥ 2 := by aesop (add simp Fact.out)
-  simp
-  
-  obtain h | h := h_isValid
-  . simp [
-      FB.not,
-      show 1 - a = (Exp.c ↑1).sub a by {
-        simp [HSub.hSub, Sub.sub, OfNat.ofNat]
-      },
-      FixedExp.eval,
-      h,
-      FB.toBool,
-      beq_eq_decide,
-      show ((0: ZMod p) = 1) = (1 = (0: ZMod p)) by grind,
-      ZMod.one_eq_zero_iff,
-      show (p = 1) = False by {
-        simp
-        omega
-      },
-      FB.ofBool,
-      FB.true
-    ]
-  . simp [
-      FB.not,
-      show 1 - a = (Exp.c ↑1).sub a by {
-        simp [HSub.hSub, Sub.sub, OfNat.ofNat]
-      },
-      FixedExp.eval,
-      h,
-      FB.toBool,
-      FB.ofBool,
-      FB.false
-    ]
+  aesop (add simp [
+    FB.not,left_inv,right_inv,toBool,FB.false,FB.true,isValid,
+    beq_eq_false_iff_ne.mpr, ofBool, FixedExp.eval
+  ])
 
 end not
 
