Clap/eDSLState/Wheels.lean
@@ -1,5 +1,7 @@
 import Lean
 
+import Mathlib.Data.ZMod.Basic
+
 @[simp]
 theorem Vector.range_one : Vector.range 1 = #v[0] := rfl
 
@@ -8,5 +10,17 @@ namespace Clap
 initialize Lean.registerTraceClass `Clap.Preprocessor
 
 initialize Lean.registerTraceClass `Clap.Preprocessor.addLambdas (inherited := true)
+
+@[simp, grind .]
+lemma ZMod.zero_ne_one
+  {p : ℕ}
+  [p_ge_2 : Fact (p ≥ 2)]
+:
+  (0: ZMod p) ≠ (1 : ZMod p)
+:= by
+  obtain ⟨p_ge_2⟩ := p_ge_2
+  symm
+  simp only [ne_eq, ZMod.one_eq_zero_iff]
+  omega
 
 end Clap
